Hs/Metatheory/Preservation2.lean
@@ -4,368 +4,14 @@ import Hs.Metatheory.Weaken
 import Hs.Metatheory.WeakenCompile
 import Hs.Metatheory.Substitution
 import Hs.Metatheory.SubstitutionCompile
+import Hs.Metatheory.Preservation1
 import SystemFD.Algorithm.Soundness2
 
-set_option maxHeartbeats 500000
-
--- Says how the shape of the core context changes with Hs Ctx
-@[aesop safe [constructors, cases]]
-inductive CompileCtx : Ctx HsTerm -> Ctx Term -> Prop where
-| nil : CompileCtx [] []
-| empty :
-  ⊢s Γ ->
-  ⊢ Γ' ->
-  CompileCtx Γ Γ' ->
-  CompileCtx (.empty :: Γ) (.empty :: Γ')
-| kind :
-  ⊢s Γ ->
-  ⊢ Γ' ->
-  CompileCtx Γ Γ' ->
-  (j1 : Γ ⊢κ A : `□) ->
-  compile_kind Γ A `□ j1 = .some A' ->
-  CompileCtx (.kind A :: Γ) (.kind A' :: Γ')
-| datatype :
-  ⊢s Γ ->
-  ⊢ Γ' ->
-  CompileCtx Γ Γ' ->
-  (j1 : Γ ⊢κ A : `□) ->
-  compile_kind Γ A `□ j1 = .some A' ->
-  CompileCtx (.datatype A :: Γ) (.datatype A' :: Γ')
-| type :
-  ⊢s Γ ->
-  ⊢ Γ' ->
-  CompileCtx Γ Γ' ->
-  (j1 : Γ ⊢τ A : `★) ->
-  compile_type Γ A `★ j1 = .some A' ->
-  CompileCtx (.type A :: Γ) (.type A' :: Γ')
-| ctor :
-  ⊢s Γ ->
-  ⊢ Γ' ->
-  CompileCtx Γ Γ' ->
-  (j1 : Γ ⊢τ A : `★) ->
-  compile_type Γ A `★ j1 = .some A' ->
-  CompileCtx (.ctor A :: Γ) (.ctor A' :: Γ')
-| term :
-  ⊢s Γ ->
-  ⊢ Γ' ->
-  CompileCtx Γ Γ' ->
-  (j1 : Γ ⊢τ A : `★)  ->
-  (j2 : Γ ⊢t t : τ) ->
-  compile_type Γ A `★ j = .some A' ->
-  compile_term Γ t τ j2 = .some t' ->
-  CompileCtx (.term A t :: Γ) (.term A' t' :: Γ')
-| openm :
-  ⊢s Γ ->
-  ⊢ Γ' ->
-  CompileCtx Γ Γ' ->
-  (j1 : Γ ⊢τ A : `★) ->
-  compile_type Γ A `★ j1 = .some A' ->
-  CompileCtx (.openm A :: Γ) (.openm A' :: Γ')
-
-theorem ctx_shift (Γ : Ctx HsTerm) :
-  (f :: Γ)d@(n + 1) = .datatype k ->
-  ∃ k', (Γ d@ n) = .datatype k' := by
-intro h;
-unfold dnth at h; unfold Frame.apply at h;
-generalize fh : Γ d@n = f at *;
-cases f;
-all_goals (simp at h)
-case _ a => exists a
-
-theorem compile_ctx_shape :
-  CompileCtx Γ Γ' ->
-  (Γ d@ x) = .datatype k ->
-  ∃ k', (Γ' d@ x) = .datatype k' := by
-intro cc h;
-induction cc;
-case _ => cases h
-case _ Γ Γ' wf wf' cc ih =>
-  cases x;
-  case _ => unfold dnth at h; cases h
-  case _ =>
-    have lem := ctx_shift Γ h
-    cases lem; case _ lem =>
-    sorry
-case _ => sorry
-case _ => sorry
-case _ => sorry
-case _ => sorry
-case _ => sorry
-case _ => sorry
-
-
-theorem compile_preserves_kinds :
-  ⊢ Γ' ->
-  (j : Γ ⊢κ t : τ) ->
-  compile_kind Γ t τ j = .some t' ->
-  Γ' ⊢ t' : .kind := by
- intro cc j c;
- induction Γ, t, τ, j using compile_kind.induct generalizing t'
- all_goals try (cases e)
- case _ =>
-   unfold compile_kind at c; cases c;
-   case _ =>
-     apply Judgment.ax; assumption;
- case _ j1 j2 ih1 ih2 =>
-   unfold compile_kind at c; simp at c;
-   rw[Option.bind_eq_some] at c;
-   cases c; case _ w1 c1 =>
-   cases c1; case _ c1 c2 =>
-   rw[Option.bind_eq_some] at c2;
-   cases c2; case _ w2 c2 =>
-   cases c2; case _ c2 c3 =>
-   cases c3;
-   have ih1' := ih1 c1;
-   have ih2' := ih2 c2;
-   apply Judgment.allk;
-   apply ih1';
-   apply ih2'
-
-theorem compile_preserves_kind_indices :
-  (∀ Γ (h1 h2 : ⊢s Γ), h1 = h2) ->
-  CompileCtx Γ Γ' ->
-  (Γ d@ x).is_datatype || (Γ d@ x).is_kind ->
-  (j : Γ ⊢κ k : s) ->
-  (Γ d@ x).get_type = .some k ->
-  compile_kind Γ k s j = .some k' ->
-  (Γ' d@ x).get_type = .some k' := by
-intro h' cc t j gt c;
-sorry
--- induction Γ, k, s, j using compile_kind.induct generalizing k'
--- case _ Γ wf =>
---   unfold compile_kind at c; cases c;
---   induction cc generalizing x <;> simp at *
---   case _ =>
---     cases t;
---     case _ t => cases t
---     case _ t => cases t
---   case _ ih =>
---     cases t;
---     case _ t =>
---       cases wf; case _ wf =>
---       have ih' := @ih (x - 1) sorry sorry sorry
---       sorry
---     case _ => sorry
---   case _ => sorry
---   case _ => sorry
---   case _ => sorry
---   case _ => sorry
--- case _ => sorry
-
-
-
--- have lem := well_sorted_kind_inversion j; cases lem
--- induction x generalizing Γ Γ' <;> simp at *;
--- case _ =>
---   unfold Frame.get_type at gt;
---   cases t;
---   case _ h =>
---     have lem := datatype_indexing_exists h;
---     cases lem; case _ w h =>
---     rw [h] at gt; simp at gt; cases gt; unfold Frame.get_type;
---     cases cc <;> cases h; unfold dnth; unfold Frame.apply; simp;
---     case _ wf wf' cc ja ca =>
---     have lem1 := hs_weaken_kind (HsJudgment.wfdatatype ja wf) ja
---     have lem2 := weaken_compile_kind ja lem1 ca
---     apply compile_kind_uniqueness h' lem1 j lem2 c;
---   case _ h =>
---     have lem := kind_indexing_exists h;
---     cases lem; case _ w h =>
---     rw [h] at gt; simp at gt; cases gt; unfold Frame.get_type;
---     cases cc <;> cases h; unfold dnth; unfold Frame.apply; simp;
---     case _ wf wf' cc ja ca =>
---     have lem1 := hs_weaken_kind (HsJudgment.wfkind ja wf) ja
---     have lem2 := weaken_compile_kind ja lem1 ca
---     apply compile_kind_uniqueness h' lem1 j lem2 c;
--- case _ ih =>
---   have ih' := @ih (.empty :: Γ) (.empty :: Γ')
---   sorry
-
-
--- theorem compile_preserves_kind_shape :
---   ⊢ Γ' ->
---   (∀ Γ (h1 h2 : ⊢s Γ), h1 = h2) ->
---   (j1 : Γ ⊢κ A : `□) ->
---   (j2 : Γ ⊢κ B : `□) ->
---   (j3 : Γ ⊢κ (A `-k> B) : `□) ->
---   compile_kind Γ A `□ j1 = .some A' ->
---   compile_kind Γ B `□ j2 = .some B' ->
---   compile_kind Γ (A `-k> B) `□ j3 = .some t' ->
---   t' = (A' -k> B') := by
--- intro wf h j1 j2 j3 c1 c2 c3;
--- have c3' := c3;
--- unfold compile_kind at c3; cases j3;
--- case _ ja jb =>
--- simp at c3;
--- rw[Option.bind_eq_some] at c3;
--- cases c3; case _ w1 c3 =>
--- cases c3; case _ c3 c4 =>
--- rw[Option.bind_eq_some] at c4;
--- cases c4; case _ w2 c4 =>
--- cases c4; case _ c4 c5 =>
--- cases c5;
--- have u := kinds_compiling_uniqueness h j1 ja c1 c3; cases u;
--- have u := kinds_compiling_uniqueness h j2 jb c2 c4; cases u;
--- simp
-
-theorem compile_preserves_types :
-  CompileCtx Γ Γ' ->
-  ⊢ Γ' ->
-  (∀ Γ (h1 h2 : ⊢s Γ), h1 = h2) ->
-  (j2 : Γ ⊢κ k : `□) ->
-  compile_kind Γ k `□ j2 = .some k' ->
-  (j1 : Γ ⊢τ τ : k) ->
-  compile_type Γ τ k j1 = .some τ' ->
-  Γ' ⊢ τ' : k' := by
-intro cc wf h j1 c1 j2 c2;
-induction Γ, τ, k, j2 using compile_type.induct generalizing Γ' τ' k'
-all_goals (unfold compile_type at c2; simp at c2)
-case _ Γ T x wf' test gt j =>
-  rw[Option.bind_eq_some] at c2;
-  cases c2; case _ w c2 =>
-  cases c2; case _ c2 e =>
-  cases e;
-  have lem := kinds_have_unique_judgments h j j1; cases lem;
-  rw[c1] at c2; cases c2;
-  have lem := Eq.symm (compile_preserves_kind_indices h cc test j (Eq.symm gt) c1)
-  apply Judgment.var; assumption; assumption
-
-case _ Γ B f A a  h1 h2 ja jb ih1 ih2 =>
-  rw[Option.bind_eq_some] at c2;
-  cases c2; case _ w1 c2 =>
-  cases c2; case _ c2 c3 =>
-  rw[Option.bind_eq_some] at c3;
-  cases c3; case _ w2 c3 =>
-  cases c3; case _ c3 c4 =>
-  rw[Option.bind_eq_some] at c4;
-  cases c4; case _ w3 c4 =>
-  cases c4; case _ c4 c5 =>
-  rw[Option.bind_eq_some] at c5;
-  cases c5; case _ w4 c5 =>
-  cases c5; case _ c5 e =>
-  cases e;
-  apply Judgment.appk;
-  case _ =>
-    have u := compile_kind_uniqueness h j1 jb c1 c3; cases u;
-    have h' : compile_kind Γ (A `-k> B) `□ (ja.arrowk jb) = some (w1 -k> k') := by
-      unfold compile_kind; simp;
-      rw[Option.bind_eq_some];
-      exists w1; apply And.intro
-      case _ => assumption
-      case _ => rw[Option.bind_eq_some]; simp; assumption
-    have ih1' := @ih1 Γ' (w1 -k> k') w3 cc wf (HsJudgment.arrowk ja jb) h' c4
-    apply ih1';
-  case _ =>
-    apply @ih2 Γ' w1 w4 cc wf ja c2 c5
-
-case _ h1 h2 ih1 =>
-  rw[Option.bind_eq_some] at c2;
-  cases c2; case _ w1 c2 =>
-  cases c2; case _ c2 c3 =>
-  rw[Option.bind_eq_some] at c3;
-  cases c3; case _ w2 c3 =>
-  cases c3; case _ c3 e =>
-  cases e; unfold compile_kind at c1; cases j1;
-  simp at c1; cases c1;
-  apply Judgment.allt;
-  apply compile_preserves_kinds wf h1 c2;
-  apply @ih1 (.kind w1 :: Γ') ★ w2 _ _ _ _ c3
-  case _ => apply CompileCtx.kind; assumption; assumption; assumption; assumption
-  case _ => apply Judgment.wfkind; apply compile_preserves_kinds wf h1 c2; assumption
-  case _ => apply HsJudgment.ax; apply HsJudgment.wfkind; assumption; assumption
-  case _ => unfold compile_kind; rfl
-
-case _ A B j1' j2' ih1 ih2 =>
-  rw[Option.bind_eq_some] at c2;
-  cases c2; case _ w1 c2 =>
-  cases c2; case _ c2 c3 =>
-  rw[Option.bind_eq_some] at c3;
-  cases c3; case _ w2 c3 =>
-  cases c3; case _ c3 e =>
-  cases e;
-  have lem1 := compile_preserves_kinds wf j1 c1;
-  unfold compile_kind at c1; simp at c1;
-  cases j1; simp at c1; cases c1;
-  apply Judgment.arrow;
-  apply @ih1 Γ' ★ w1 cc wf _ _ c2;
-  case _ => apply HsJudgment.ax; assumption
-  case _ => unfold compile_kind; rfl
-
-  apply @ih2 (.empty::Γ') ★ w2 _ _ _ _ c3;
-  case _ => apply CompileCtx.empty; assumption; assumption; assumption
-  case _ => apply Judgment.wfempty; assumption;
-  case _ => apply HsJudgment.ax; apply HsJudgment.wfempty; assumption
-  case _ => unfold compile_kind; rfl
-
-case _ j1 _ j2 ih1 ih2 =>
-  rw[Option.bind_eq_some] at c2;
-  cases c2; case _ w1 c2 =>
-  cases c2; case _ c2 c3 =>
-  rw[Option.bind_eq_some] at c3;
-  cases c3; case _ w2 c3 =>
-  cases c3; case _ c3 e =>
-  cases e;
-  have lem1 := compile_preserves_kinds wf j1 c1;
-  unfold compile_kind at c1; simp at c1;
-  cases j1; simp at c1; cases c1;
-  case _ tl1 tl2 _ =>
-  apply Judgment.arrow;
-  apply @ih1 Γ' ★ w1 cc wf _ _ c2;
-  case _ => apply HsJudgment.ax; assumption
-  case _ => unfold compile_kind; rfl
-  apply @ih2 (.empty::Γ') ★ w2 _ _ _ _ c3
-  case _ => apply CompileCtx.empty; assumption; assumption; assumption
-  case _ => apply Judgment.wfempty; assumption
-  case _ => apply HsJudgment.ax; apply HsJudgment.wfempty; assumption
-  case _ => unfold compile_kind; rfl
-
-
-@[simp]
-abbrev CompilePreservesTypeShapeAll :  (v : HsVariant) -> Ctx HsTerm -> HsJudgmentArgs v -> Prop
-| .type => λ Γ => λ (τ, k) => ∀ wA wτ cτ,
-  τ = (`∀{wA} wτ) ->
-  k = `★ ->
-  (j3 : Γ ⊢τ τ : k) ->
-  compile_type Γ τ k j3 = .some cτ ->
-  ∃ A' τ', cτ = ∀[A']τ'
-| _ => λ _ => λ _ => true
-
-theorem comile_preserves_type_shape_all_lemma :
-  HsJudgment v Γ idx -> CompilePreservesTypeShapeAll v Γ idx
- := by
-intro j; induction j <;> simp at *;
-intro wA wτ cτ e1 e2 j3 c3;
-cases j3; case _ hka hkb =>
-unfold compile_type at c3; simp at c3;
-rw[Option.bind_eq_some] at c3;
-cases c3; case _ A' c3 =>
-cases c3; case _ cA c4 =>
-rw[Option.bind_eq_some] at c4;
-cases c4; case _ B' c4 =>
-cases c4; case _ cB e =>
-cases e; simp;
-
-theorem compile_preserves_type_shape_all :
-  (j : Γ ⊢τ (`∀{A}τ) : `★) ->
-  compile_type Γ (`∀{A}τ) `★ j = .some cτ ->
-  ∃ A' τ', cτ = ∀[A']τ' := by
-intro j c;
-have lem := comile_preserves_type_shape_all_lemma j; simp at lem;
-apply @lem A τ cτ rfl rfl j c
-
-
-theorem compile_preserves_type_indices :
-  (∀ Γ (h1 h2 : ⊢s Γ), h1 = h2) ->
-  CompileCtx Γ Γ' ->
-  (Γ d@ x).is_ctor || (Γ d@ x).is_term || (Γ d@ x).is_type ->
-  (j : Γ ⊢τ T : k) ->
-  (Γ d@ x).get_type = .some T ->
-  compile_type Γ T k j = .some T' ->
-  (Γ' d@ x).get_type = .some T' := by sorry
+set_option maxHeartbeats 5000000
 
 theorem compile_preserves_terms :
   (∀ Γ (h1 h2 : ⊢s Γ), h1 = h2) ->
-  CompileCtx Γ Γ' ->
+  (∀ v, CompileCtxPred v) ->
   ⊢ Γ' ->
   (j1 : Γ ⊢τ τ : k) ->
   compile_type Γ τ k j1 = .some τ' ->
@@ -375,12 +21,11 @@ theorem compile_preserves_terms :
 intro h cc wf j1 c1 j2 c2;
 induction Γ, t, τ, j2 using compile_term.induct generalizing Γ' t' τ' k
 all_goals (unfold compile_term at c2; simp at c2)
-case _ wf test gt =>
-     cases c2;
-     apply Judgment.var;
-     assumption;
-     have lem := compile_preserves_type_indices h cc test j1 (Eq.symm gt) c1;
-     apply Eq.symm lem
+case _ τ Γ x wf' test gt =>
+     cases c2; simp at cc;
+     have lem := @cc .type Γ Γ' x k τ τ' wf' (Eq.symm gt) j1 c1
+     symm at lem;
+     apply Judgment.var; assumption; assumption
 
 case _ Γ A t B j1' j2 j3 ih1 => -- lam
  rw[Option.bind_eq_some] at c2;
@@ -393,7 +38,6 @@ case _ Γ A t B j1' j2 j3 ih1 => -- lam
  cases c4; case _ t' c4 =>
  cases c4; case _ c4 e =>
  cases e;
- -- have uniq := types_have_unique_kinds j1 j3; subst uniq;
  unfold compile_type at c1; cases j1; simp at c1;
  rw[Option.bind_eq_some] at c1;
  cases c1; case _ x1 c1' =>
@@ -402,88 +46,151 @@ case _ Γ A t B j1' j2 j3 ih1 => -- lam
  cases c2'; case _ B' c2' =>
  cases c2'; case _ c2' e =>
  cases e; case _ ja jb =>
- have cc' : CompileCtx (.type A :: Γ) (.type A' :: Γ') := by
-   apply CompileCtx.type;
-   apply hs_judgment_ctx_wf .type j1'
-   apply wf
-   apply cc
-   apply c2
- have wf' : ⊢ (.type A' :: Γ') := by
-   apply Judgment.wftype
-   apply compile_preserves_types cc wf h _ _ j1' c2
-   case _ => apply HsJudgment.ax (hs_judgment_ctx_wf .type ja)
-   case _ => unfold compile_kind; rfl
-   assumption
  have lem := compile_type_uniqueness h j1' ja c2 c1'; cases lem;
+ have lem := compile_type_uniqueness h jb j3 c2' c3; cases lem;
  apply Judgment.lam;
- apply compile_preserves_types cc wf h _ _ ja c1'
+ apply compile_preserves_types (cc .kind) wf h _ _ ja c1'
  case _ => apply HsJudgment.ax (hs_judgment_ctx_wf .type ja)
  case _ => unfold compile_kind; rfl
  case _ =>
-   have ih1' := @ih1 (.type A' :: Γ') `★ B' t' cc' wf'
-   sorry
- apply compile_preserves_types cc wf h _ _ _ _
- case _ => apply `★;
- case _ => apply (A → B)
- case _ => apply HsJudgment.ax (hs_judgment_ctx_wf .type ja)
- case _ => unfold compile_kind; rfl
- case _ => apply HsJudgment.arrow; assumption; assumption
+   have j' := (hs_replace_empty_type ja jb)
+   have lem := compile_replace_empty jb j' c2'
+   apply @ih1 (.type A' :: Γ') `★ B' t' _ j' lem c4
+   apply Judgment.wftype
+   apply compile_preserves_types (cc .kind) wf h _ _ j1' c2
+   case _ => apply HsJudgment.ax (hs_judgment_ctx_wf .type j1')
+   case _ => unfold compile_kind; rfl
+   apply wf
  case _ =>
-   unfold compile_type; simp;
-   rw[Option.bind_eq_some]; exists A';
-   apply And.intro; assumption;
-   rw[Option.bind_eq_some]; exists B';
+   apply Judgment.arrow;
+   apply compile_preserves_types (cc .kind) wf h _ _ j1' c2
+   case _ => apply HsJudgment.ax (hs_judgment_ctx_wf .type j1')
+   case _ => unfold compile_kind; rfl
+   have u := types_have_unique_judgments h j3 jb; cases u
+   have lem1' := Judgment.wfempty wf
+   have lem1 := HsJudgment.wfempty (hs_judgment_ctx_wf .type ja)
+   have lem2 := HsJudgment.ax (hs_judgment_ctx_wf .type ja)
+   apply compile_preserves_types (cc .kind) _ h _ _ j3 c3;
+   case _ => apply lem1'
+   case _ => have lem := hs_weaken_empty_kind lem2; simp at lem; apply lem
+   case _ =>
+     unfold hs_weaken_empty_kind; unfold hs_weaken_kind; cases lem2;
+     unfold hs_judgment_ctx_wf; simp;
+     unfold hs_rename; simp; unfold compile_kind; rfl
 
-case _ h1 h2 ih1 ih2 =>
+case _ Γ t1 A B t2 h1 h2 h3 h4 ih1 ih2 => -- app
  rw[Option.bind_eq_some] at c2;
- cases c2; case _ wt1 c2 =>
+ cases c2; case _ AB' c2 =>
  cases c2; case _ c2 c3 =>
  rw[Option.bind_eq_some] at c3;
- cases c3; case _ wt2 c3 =>
- cases c3; case _ c3 e =>
- cases e;
- apply Judgment.app;
- sorry
- case _ =>
-   have ih2' := @ih2 Γ' `★
-   sorry
- sorry
- sorry
- sorry
-
-case _ =>
- sorry
-case _ =>
- rw[Option.bind_eq_some] at c2;
- cases c2; case _ wt1 c2 =>
- cases c2; case _ c2 c3 =>
- rw[Option.bind_eq_some] at c3;
- cases c3; case _ wt2 c3 =>
+ cases c3; case _ A' c3 =>
  cases c3; case _ c3 c4 =>
  rw[Option.bind_eq_some] at c4;
- cases c4; case _ wt3 c4 =>
+ cases c4; case _ wB' c4 =>
  cases c4; case _ c4 c5 =>
  rw[Option.bind_eq_some] at c5;
- cases c5; case _ wt4 c5 =>
- cases c5; case _ c5 e =>
+ cases c5; case _ t1' c5 =>
+ cases c5; case _ c5 c6 =>
+ rw[Option.bind_eq_some] at c6;
+ cases c6; case _ t2' c6 =>
+ cases c6; case _ c6 e =>
  cases e;
+ have u := types_have_unique_kinds j1 h4; cases u;
+ have lem := compile_preserves_type_shape_arrow (extract_typing h1) c2
+ cases lem; case _ wA lem =>
+ cases lem; case _ wB lem  =>
+ cases lem; case _ ja' lem =>
+ cases lem; case _ jb' lem =>
+ cases lem; case _ e lem =>
+ cases lem; case _ c1' c2' =>
+   cases e;
+   have lem := compile_type_uniqueness h h3 ja' c3 c1'; cases lem
+   have lem := compile_beta_empty_term jb' c2' h2 c6 (hs_beta_empty_type t2 jb');
+   have lem' := compile_type_uniqueness h (hs_beta_empty_type t2 jb') j1 lem c1
+   apply Judgment.app;
+   case _ =>
+     have ih' := @ih1 Γ' `★ (A' -t> wB) t1' wf (extract_typing h1) c2 c5;
+     apply ih'
+   case _ =>
+     have ih' :=  @ih2 Γ' `★ A' t2' wf h3 c3 c6
+     apply ih'
+   symm at lem'; apply lem'
+
+case _ B Γ A t1 t2 j1' j2 j3 j4 ih1 ih2 => -- letterm
+ rw[Option.bind_eq_some] at c2;
+ cases c2; case _ A' c2 =>
+ cases c2; case _ c2 c3 =>
+ rw[Option.bind_eq_some] at c3;
+ cases c3; case _ t1' c3 =>
+ cases c3; case _ c3 c4 =>
+ rw[Option.bind_eq_some] at c4;
+ cases c4; case _ t2' c4 =>
+ cases c4; case _ c4 e =>
+ cases e;
+ have lemA : Γ' ⊢ A' : ★ := by
+   apply compile_preserves_types (cc .kind) wf h _ _ j1' c2;
+   apply HsJudgment.ax (hs_judgment_ctx_wf .type j1')
+   unfold compile_kind; rfl
+ have lemt1 := @ih1 Γ' `★ A' t1' wf j1' c2 c3
+ have lem := types_have_unique_kinds j1 j4; cases lem;
+ have lemΓ' := by apply Judgment.wfterm; assumption; assumption; assumption
+ have lemΓ : ⊢s (.term A t1 :: Γ) := by apply HsJudgment.wfterm; assumption; assumption; (apply hs_judgment_ctx_wf .type j1')
+ apply Judgment.letterm;
+ case _ => assumption
+ case _ => assumption
+ case _ =>
+   apply @ih2 (.term A' t1' :: Γ') `★ ([S]τ') t2' _ _ _ c4;
+   case _ => assumption
+   case _ => apply hs_weaken_type lemΓ j1
+   case _ => apply weaken_compile_type j1 c1
+ case _ =>
+   apply compile_preserves_types (cc .kind) wf h _ _ _ c1;
+   apply HsJudgment.ax (hs_judgment_ctx_wf .type j1)
+   unfold compile_kind; rfl
+case _ T Γ A R B p s i t jA jR jB jT jp js ji jt j9 j10 j11 j12 ih1 ih2 ih3 ih4 =>
+ have u := types_have_unique_kinds jT j1; cases u;
+ rw[Option.bind_eq_some] at c2;
+ cases c2; case _ wA c2 =>
+ cases c2; case _ c2 c3 =>
+ rw[Option.bind_eq_some] at c3;
+ cases c3; case _ wR c3 =>
+ cases c3; case _ c3 c4 =>
+ rw[Option.bind_eq_some] at c4;
+ cases c4; case _ wB c4 =>
+ cases c4; case _ c4 c5 =>
+ rw[Option.bind_eq_some] at c5;
+ cases c5; case _ wT c5 =>
+ cases c5; case _ c5 c6 =>
+ rw[Option.bind_eq_some] at c6;
+ cases c6; case _ wp c6 =>
+ cases c6; case _ c6 c7 =>
+ rw[Option.bind_eq_some] at c7;
+ cases c7; case _ ws c7 =>
+ cases c7; case _ c7 c8 =>
+ rw[Option.bind_eq_some] at c8;
+ cases c8; case _ wi c8 =>
+ cases c8; case _ c8 c9 =>
+ rw[Option.bind_eq_some] at c9;
+ cases c9; case _ wt c9 =>
+ cases c9; case _ c9 e =>
+ cases e;
+ have lemAx : Γ ⊢κ `★ : `□ := by apply HsJudgment.ax (hs_judgment_ctx_wf .type jA)
+ have lemK : compile_kind Γ `★ `□ lemAx = .some ★ := by unfold compile_kind; cases lemAx; simp
  apply Judgment.ite;
+ apply @ih1 Γ' `★ wA wp wf jA c2 c6
+ apply @ih2 Γ' `★ wR ws wf jR c3 c7
+ apply compile_preserves_types (cc .kind) wf h lemAx lemK jR c3
+ apply @ih3 Γ' `★ wB wi wf jB c4 c8;
  sorry
  sorry
  sorry
  sorry
- sorry
- sorry
- sorry
- sorry
- sorry
- sorry
- sorry
- sorry
- sorry
+ apply compile_preserves_types (cc .kind) wf h lemAx lemK j1 c1
+ apply @ih4 Γ' `★ τ' wt wf j1 c1
+ apply c9
 
 -- implicits
-case _ Γ t A τ e h1 h2 h3 h4 ih => -- implicitAllE
+case _ Γ t A τ e h1 h2 h3 h4 h5 ih => -- implicitAllE
  rw[Option.bind_eq_some] at c2;
  cases c2; case _ wτ c2 =>
  cases c2; case _ c2 c3 =>
@@ -503,10 +210,10 @@ case _ Γ t A τ e h1 h2 h3 h4 ih => -- implicitAllE
  cases lem;
  apply Judgment.appt;
  case _ => --
-   have ih' := @ih Γ' `★ (∀[A']τ') wt cc wf h1 c2 c4;
+   have ih' := @ih Γ' `★ (∀[A']τ') wt wf h1 c2 c4;
    apply ih'
  case _ =>
-   have h' := compile_preserves_types cc wf h h2 c3 h4 c5
+   have h' := compile_preserves_types (cc .kind) wf h h2 c3 h4 c5
    unfold compile_type at c2; cases h1; simp at c2;
    rw[Option.bind_eq_some] at c2;
    cases c2; case _ wA' c2' =>
@@ -518,7 +225,7 @@ case _ Γ t A τ e h1 h2 h3 h4 ih => -- implicitAllE
    have lem := compile_kind_uniqueness h h2 h2' c3 c2'; cases lem;
    assumption
  case _ =>
-   have h' := compile_preserves_types cc wf h h2 c3 h4 c5
+   have h' := compile_preserves_types (cc .kind) wf h h2 c3 h4 c5
    unfold compile_type at c2; cases h1; simp at c2;
    rw[Option.bind_eq_some] at c2;
    cases c2; case _ wA' c2' =>
@@ -556,20 +263,16 @@ case _ Γ t A τ j1' j2 j3 ih =>
   cases e;
   have u := kinds_have_unique_judgments h ja' j2; cases u;
   rw[c1] at c3; cases c3;
-  have cc' : CompileCtx (.kind A::Γ) (.kind wA :: Γ') := by
-    apply CompileCtx.kind _ wf cc;
-    case _ => apply c1
-    apply hs_judgment_ctx_wf .kind j2
   have lem : ⊢ (.kind wA :: Γ') := by
     apply Judgment.wfkind;
     apply compile_preserves_kinds wf j2 c1; assumption
   apply Judgment.lamt;
   apply compile_preserves_kinds wf j2 c1
-  apply @ih (Frame.kind wA :: Γ') `★ wt' wt cc' lem j1 c2' c2;
+  apply @ih (Frame.kind wA :: Γ') `★ wt' wt lem j1 c2' c2;
   case _ =>
     apply Judgment.allt;
     apply compile_preserves_kinds wf j2 c1;
-    apply compile_preserves_types cc' lem h _ _ j1 c2'
+    apply compile_preserves_types (cc .kind) lem h _ _ j1 c2'
     case _ =>
       apply HsJudgment.ax;
       apply HsJudgment.wfkind; assumption
@@ -577,8 +280,68 @@ case _ Γ t A τ j1' j2 j3 ih =>
     case _ =>
       unfold compile_kind; rfl;
 
-case _ => sorry
-case _ => sorry
+case _ Γ t π τ j1' j2 j4 j3 ih1 => -- implicitArrI
+ rw[Option.bind_eq_some] at c2;
+ cases c2; case _ π' c2 =>
+ cases c2; case _ c2 c3 =>
+ rw[Option.bind_eq_some] at c3;
+ cases c3; case _ t' c3 =>
+ cases c3; case _ c3 e =>
+ cases e;
+ unfold compile_type at c1; cases j1; simp at c1;
+ rw[Option.bind_eq_some] at c1;
+ cases c1; case _ x1 c1' =>
+ cases c1'; case _ c1' c2' =>
+ rw[Option.bind_eq_some] at c2';
+ cases c2'; case _ B' c2' =>
+ cases c2'; case _ c2' e =>
+ cases e; case _ ja _ jb =>
+ have lem := compile_type_uniqueness h j1' ja c2 c1'; cases lem;
+ -- have lem := compile_type_uniqueness h jb j2 c2' c3; cases lem;
+ apply Judgment.lam;
+ apply compile_preserves_types (cc .kind) wf h _ _ ja c1'
+ case _ => apply HsJudgment.ax (hs_judgment_ctx_wf .type ja)
+ case _ => unfold compile_kind; rfl
+ case _ =>
+   have j' := (hs_replace_empty_type ja jb)
+   have lem := compile_replace_empty jb j' c2'
+   apply @ih1 (.type π' :: Γ') `★ B' t' _ j' lem c3
+   apply Judgment.wftype
+   apply compile_preserves_types (cc .kind) wf h _ _ j1' c2
+   case _ => apply HsJudgment.ax (hs_judgment_ctx_wf .type j1')
+   case _ => unfold compile_kind; rfl
+   apply wf
+ case _ =>
+   apply Judgment.arrow;
+   apply compile_preserves_types (cc .kind) wf h _ _ j1' c2
+   case _ => apply HsJudgment.ax (hs_judgment_ctx_wf .type j1')
+   case _ => unfold compile_kind; rfl
+   have lem1' := Judgment.wfempty wf
+   have lem1 := HsJudgment.wfempty (hs_judgment_ctx_wf .type ja)
+   have lem2 := HsJudgment.ax (hs_judgment_ctx_wf .type ja)
+   apply compile_preserves_types (cc .kind) _ h _ _ jb c2';
+   case _ => apply lem1'
+   case _ => have lem := hs_weaken_empty_kind lem2; simp at lem; apply lem
+   case _ =>
+     unfold hs_weaken_empty_kind; unfold hs_weaken_kind; cases lem2;
+     unfold hs_judgment_ctx_wf; simp;
+     unfold hs_rename; simp; unfold compile_kind; rfl
+case _ => -- implicitArrE
+  rw[Option.bind_eq_some] at c2;
+  cases c2; case _ wt c2 =>
+  cases c2; case _ c2 c3 =>
+  rw[Option.bind_eq_some] at c3;
+  cases c3; case _ we c3 =>
+  cases c3; case _ c3 e =>
+  cases e;
+  apply Judgment.app;
+  sorry
+  sorry
+  sorry
+  sorry
+  sorry
+
+
 
 ---------------------------------------------
 -- Contexts
@@ -662,111 +425,111 @@ case _ => sorry
 case _ => sorry
 
 
-theorem cc_soundness Γ : ⊢s Γ -> (Η : HsCtx Γ) -> compile_ctx Η = .some Γ' -> CompileCtx Γ Γ'
-  := by
-intro wf h j
-induction h using compile_ctx.induct generalizing Γ'
-case _ =>
-  unfold compile_ctx at j; cases j;
-  constructor;
-case _ Γ Η ih =>
-  unfold compile_ctx at j; simp at j;
-  rw[Option.bind_eq_some] at j;
-  cases j; case _ w j =>
-  cases j; case _ j j1 =>
-  rw[Option.bind_eq_some] at j1;
-  cases j1; case _ w1 j1 =>
-  cases j1; case _ j1 e =>
-  cases e; cases wf; case _ wf =>
-  apply CompileCtx.empty;
-  assumption
-  apply compile_preserves_wf Γ wf Η j
-  apply ih wf j
-case _ Γ k Η jk ih =>
-  unfold compile_ctx at j; simp at j;
-  rw[Option.bind_eq_some] at j;
-  cases j; case _ w j =>
-  cases j; case _ j j1 =>
-  rw[Option.bind_eq_some] at j1;
-  cases j1; case _ w1 j1 =>
-  cases j1; case _ j1 j2 =>
-  rw[Option.bind_eq_some] at j2;
-  cases j2; case _ w2 j2 =>
-  cases j2; case _ j2 e =>
-  cases e; cases wf; case _ wf jk' =>
-  apply CompileCtx.kind;
-  assumption
-  apply compile_preserves_wf Γ wf Η j
-  apply ih wf j
-  assumption
-case _ Γ k Η jk ih =>
-  unfold compile_ctx at j; simp at j;
-  rw[Option.bind_eq_some] at j;
-  cases j; case _ w j =>
-  cases j; case _ j j1 =>
-  rw[Option.bind_eq_some] at j1;
-  cases j1; case _ w1 j1 =>
-  cases j1; case _ j1 j2 =>
-  rw[Option.bind_eq_some] at j2;
-  cases j2; case _ w2 j2 =>
-  cases j2; case _ j2 e =>
-  cases e; cases wf; case _ wf jk' =>
-  apply CompileCtx.datatype;
-  assumption
-  apply compile_preserves_wf Γ wf Η j
-  apply ih wf j
-  assumption
-case _  Γ k Η _ ih =>
-  unfold compile_ctx at j; simp at j;
-  rw[Option.bind_eq_some] at j;
-  cases j; case _ w j =>
-  cases j; case _ j j1 =>
-  rw[Option.bind_eq_some] at j1;
-  cases j1; case _ w1 j1 =>
-  cases j1; case _ j1 j2 =>
-  rw[Option.bind_eq_some] at j2;
-  cases j2; case _ w2 j2 =>
-  cases j2; case _ j2 e =>
-  cases e; cases wf; case _ wf jk' =>
-  apply CompileCtx.type;
-  assumption
-  apply compile_preserves_wf Γ wf Η j
-  apply ih wf j
-  assumption
-case _  Γ k Η _ ih =>
-  unfold compile_ctx at j; simp at j;
-  rw[Option.bind_eq_some] at j;
-  cases j; case _ w j =>
-  cases j; case _ j j1 =>
-  rw[Option.bind_eq_some] at j1;
-  cases j1; case _ w1 j1 =>
-  cases j1; case _ j1 j2 =>
-  rw[Option.bind_eq_some] at j2;
-  cases j2; case _ w2 j2 =>
-  cases j2; case _ j2 e =>
-  cases e; cases wf; case _ wf _ vh =>
-  apply CompileCtx.ctor;
-  assumption
-  apply compile_preserves_wf Γ wf Η j
-  apply ih wf j
-  assumption
-case _  Γ k Η _ ih =>
-  unfold compile_ctx at j; simp at j;
-  rw[Option.bind_eq_some] at j;
-  cases j; case _ w j =>
-  cases j; case _ j j1 =>
-  rw[Option.bind_eq_some] at j1;
-  cases j1; case _ w1 j1 =>
-  cases j1; case _ j1 j2 =>
-  rw[Option.bind_eq_some] at j2;
-  cases j2; case _ w2 j2 =>
-  cases j2; case _ j2 e =>
-  cases e; cases wf; case _ wf jk =>
-  apply CompileCtx.openm;
-  assumption
-  apply compile_preserves_wf Γ wf Η j
-  apply ih wf j
-  assumption
+-- theorem cc_soundness Γ : ⊢s Γ -> (Η : HsCtx Γ) -> compile_ctx Η = .some Γ' -> CompileCtx Γ Γ'
+--   := by
+-- intro wf h j
+-- induction h using compile_ctx.induct generalizing Γ'
+-- case _ =>
+--   unfold compile_ctx at j; cases j;
+--   constructor;
+-- case _ Γ Η ih =>
+--   unfold compile_ctx at j; simp at j;
+--   rw[Option.bind_eq_some] at j;
+--   cases j; case _ w j =>
+--   cases j; case _ j j1 =>
+--   rw[Option.bind_eq_some] at j1;
+--   cases j1; case _ w1 j1 =>
+--   cases j1; case _ j1 e =>
+--   cases e; cases wf; case _ wf =>
+--   apply CompileCtx.empty;
+--   assumption
+--   apply compile_preserves_wf Γ wf Η j
+--   apply ih wf j
+-- case _ Γ k Η jk ih =>
+--   unfold compile_ctx at j; simp at j;
+--   rw[Option.bind_eq_some] at j;
+--   cases j; case _ w j =>
+--   cases j; case _ j j1 =>
+--   rw[Option.bind_eq_some] at j1;
+--   cases j1; case _ w1 j1 =>
+--   cases j1; case _ j1 j2 =>
+--   rw[Option.bind_eq_some] at j2;
+--   cases j2; case _ w2 j2 =>
+--   cases j2; case _ j2 e =>
+--   cases e; cases wf; case _ wf jk' =>
+--   apply CompileCtx.kind;
+--   assumption
+--   apply compile_preserves_wf Γ wf Η j
+--   apply ih wf j
+--   assumption
+-- case _ Γ k Η jk ih =>
+--   unfold compile_ctx at j; simp at j;
+--   rw[Option.bind_eq_some] at j;
+--   cases j; case _ w j =>
+--   cases j; case _ j j1 =>
+--   rw[Option.bind_eq_some] at j1;
+--   cases j1; case _ w1 j1 =>
+--   cases j1; case _ j1 j2 =>
+--   rw[Option.bind_eq_some] at j2;
+--   cases j2; case _ w2 j2 =>
+--   cases j2; case _ j2 e =>
+--   cases e; cases wf; case _ wf jk' =>
+--   apply CompileCtx.datatype;
+--   assumption
+--   apply compile_preserves_wf Γ wf Η j
+--   apply ih wf j
+--   assumption
+-- case _  Γ k Η _ ih =>
+--   unfold compile_ctx at j; simp at j;
+--   rw[Option.bind_eq_some] at j;
+--   cases j; case _ w j =>
+--   cases j; case _ j j1 =>
+--   rw[Option.bind_eq_some] at j1;
+--   cases j1; case _ w1 j1 =>
+--   cases j1; case _ j1 j2 =>
+--   rw[Option.bind_eq_some] at j2;
+--   cases j2; case _ w2 j2 =>
+--   cases j2; case _ j2 e =>
+--   cases e; cases wf; case _ wf jk' =>
+--   apply CompileCtx.type;
+--   assumption
+--   apply compile_preserves_wf Γ wf Η j
+--   apply ih wf j
+--   assumption
+-- case _  Γ k Η _ ih =>
+--   unfold compile_ctx at j; simp at j;
+--   rw[Option.bind_eq_some] at j;
+--   cases j; case _ w j =>
+--   cases j; case _ j j1 =>
+--   rw[Option.bind_eq_some] at j1;
+--   cases j1; case _ w1 j1 =>
+--   cases j1; case _ j1 j2 =>
+--   rw[Option.bind_eq_some] at j2;
+--   cases j2; case _ w2 j2 =>
+--   cases j2; case _ j2 e =>
+--   cases e; cases wf; case _ wf _ vh =>
+--   apply CompileCtx.ctor;
+--   assumption
+--   apply compile_preserves_wf Γ wf Η j
+--   apply ih wf j
+--   assumption
+-- case _  Γ k Η _ ih =>
+--   unfold compile_ctx at j; simp at j;
+--   rw[Option.bind_eq_some] at j;
+--   cases j; case _ w j =>
+--   cases j; case _ j j1 =>
+--   rw[Option.bind_eq_some] at j1;
+--   cases j1; case _ w1 j1 =>
+--   cases j1; case _ j1 j2 =>
+--   rw[Option.bind_eq_some] at j2;
+--   cases j2; case _ w2 j2 =>
+--   cases j2; case _ j2 e =>
+--   cases e; cases wf; case _ wf jk =>
+--   apply CompileCtx.openm;
+--   assumption
+--   apply compile_preserves_wf Γ wf Η j
+--   apply ih wf j
+--   assumption
 
 -- theorem cc_completeness Γ : ⊢s Γ -> (Η : HsCtx Γ) -> CompileCtx Γ Γ' -> compile_ctx Η = .some Γ'
 --   := by
