Hs/Metatheory/Uniqueness.lean
@@ -181,3 +181,39 @@ intro j; cases j; rfl
 theorem all_kind_inversion :
   Γ ⊢τ (`∀{A} B) : k -> k = `★ := by
 intro j; cases j; rfl
+
+
+@[simp]
+abbrev TypingJudgmentsUniquessType : (v : HsVariant) -> Ctx HsTerm -> HsJudgmentArgs v -> Prop
+| .term => λ Γ => λ (t, τ) =>
+   (j1 : Γ ⊢t t : τ) -> (j2 : Γ ⊢t t : τ) -> j1 = j2
+| _ => λ _ => λ _ => true
+
+theorem terms_have_unique_judgments_lemma :
+  (∀ Γ (h1 h2 : ⊢s Γ), h1 = h2) ->
+  HsJudgment v Γ idx -> TypingJudgmentsUniquessType v Γ idx := by
+intro h j; induction j <;> simp at *
+all_goals (intro j1 j2)
+case _ =>
+
+  sorry
+case _ =>
+
+  sorry
+case _ => sorry
+case _ => sorry
+case _ => sorry
+case _ => sorry
+case _ => sorry
+case _ => sorry
+case _ => sorry
+
+
+
+theorem terms_have_unique_judgments :
+  (∀ Γ (h1 h2 : ⊢s Γ), h1 = h2) ->
+  (j1 : Γ ⊢t t : k) ->
+  (j2 : Γ ⊢t t : k) ->
+  j1 = j2 := by
+intro h j1 j2;
+apply terms_have_unique_judgments_lemma h j2 j1 j2;
