Hs/Metatheory/Preservation1.lean
@@ -1,0 +1,248 @@
+import Hs.Algorithm
+import Hs.Metatheory.Uniqueness
+import Hs.Metatheory.Weaken
+import Hs.Metatheory.WeakenCompile
+import Hs.Metatheory.Substitution
+import Hs.Metatheory.SubstitutionCompile
+import SystemFD.Algorithm.Soundness2
+
+set_option maxHeartbeats 5000000
+
+theorem compile_preserves_kinds :
+  ⊢ Γ' ->
+  (j : Γ ⊢κ t : τ) ->
+  compile_kind Γ t τ j = .some t' ->
+  Γ' ⊢ t' : .kind := by
+ intro cc j c;
+ induction Γ, t, τ, j using compile_kind.induct generalizing t'
+ all_goals try (cases e)
+ case _ =>
+   unfold compile_kind at c; cases c;
+   case _ =>
+     apply Judgment.ax; assumption;
+ case _ j1 j2 ih1 ih2 =>
+   unfold compile_kind at c; simp at c;
+   rw[Option.bind_eq_some] at c;
+   cases c; case _ w1 c1 =>
+   cases c1; case _ c1 c2 =>
+   rw[Option.bind_eq_some] at c2;
+   cases c2; case _ w2 c2 =>
+   cases c2; case _ c2 c3 =>
+   cases c3;
+   have ih1' := ih1 c1;
+   have ih2' := ih2 c2;
+   apply Judgment.allk;
+   apply ih1';
+   apply ih2'
+
+
+@[simp]
+abbrev CompileCtxPred : (v : HsVariant) -> Prop
+| .kind => ∀ Γ Γ' x T T',
+  ⊢s Γ ->
+  (Γ d@ x).get_type = .some T ->
+  (j : Γ ⊢κ T : `□) ->
+  compile .kind Γ ⟨(T, `□), j⟩ = .some T' ->
+  (Γ' d@ x).get_type = .some T'
+| .type =>
+  ∀ Γ Γ' x k T T', ⊢s Γ ->
+  (Γ d@ x).get_type = .some T ->
+  (j : Γ ⊢τ T : k) ->
+  compile .type Γ ⟨(T, k), j⟩ = .some T' ->
+  (Γ' d@ x).get_type = .some T'
+| .term =>
+  ∀ Γ Γ' x T T' A, ⊢s Γ ->
+  (Γ d@ x).get_type = .some T ->
+  (j : Γ ⊢t T : A) ->
+  compile .term Γ ⟨(T, A), j⟩ = .some T' ->
+  (Γ' d@ x).get_type = .some T'
+| .ctx => true
+
+
+theorem compile_preserves_types :
+  CompileCtxPred .kind ->
+  ⊢ Γ' ->
+  (∀ Γ (h1 h2 : ⊢s Γ), h1 = h2) ->
+  (j2 : Γ ⊢κ k : `□) ->
+  compile_kind Γ k `□ j2 = .some k' ->
+  (j1 : Γ ⊢τ τ : k) ->
+  compile_type Γ τ k j1 = .some τ' ->
+  Γ' ⊢ τ' : k' := by
+intro cc wf h j1 c1 j2 c2;
+induction Γ, τ, k, j2 using compile_type.induct generalizing Γ' τ' k'
+all_goals (unfold compile_type at c2; simp at c2)
+case _ Γ T x wf' test gt j =>
+  rw[Option.bind_eq_some] at c2;
+  cases c2; case _ w c2 =>
+  cases c2; case _ c2 e =>
+  cases e;
+  have lem := kinds_have_unique_judgments h j j1; cases lem;
+  rw[c1] at c2; cases c2;
+  simp at cc;
+  have lem := @cc Γ Γ' x T k' wf' (Eq.symm gt) j c1; symm at lem;
+  apply Judgment.var; assumption; assumption
+
+case _ Γ B f A a  h1 h2 ja jb ih1 ih2 =>
+  rw[Option.bind_eq_some] at c2;
+  cases c2; case _ w1 c2 =>
+  cases c2; case _ c2 c3 =>
+  rw[Option.bind_eq_some] at c3;
+  cases c3; case _ w2 c3 =>
+  cases c3; case _ c3 c4 =>
+  rw[Option.bind_eq_some] at c4;
+  cases c4; case _ w3 c4 =>
+  cases c4; case _ c4 c5 =>
+  rw[Option.bind_eq_some] at c5;
+  cases c5; case _ w4 c5 =>
+  cases c5; case _ c5 e =>
+  cases e;
+  apply Judgment.appk;
+  case _ =>
+    have u := compile_kind_uniqueness h j1 jb c1 c3; cases u;
+    have h' : compile_kind Γ (A `-k> B) `□ (ja.arrowk jb) = some (w1 -k> k') := by
+      unfold compile_kind; simp;
+      rw[Option.bind_eq_some];
+      exists w1; apply And.intro
+      case _ => assumption
+      case _ => rw[Option.bind_eq_some]; simp; assumption
+    have ih1' := @ih1 Γ' (w1 -k> k') w3 wf (HsJudgment.arrowk ja jb) h' c4
+    apply ih1';
+  case _ =>
+    apply @ih2 Γ' w1 w4 wf ja c2 c5
+
+case _ h1 h2 ih1 =>
+  rw[Option.bind_eq_some] at c2;
+  cases c2; case _ w1 c2 =>
+  cases c2; case _ c2 c3 =>
+  rw[Option.bind_eq_some] at c3;
+  cases c3; case _ w2 c3 =>
+  cases c3; case _ c3 e =>
+  cases e; unfold compile_kind at c1; cases j1;
+  simp at c1; cases c1;
+  apply Judgment.allt;
+  apply compile_preserves_kinds wf h1 c2;
+  apply @ih1 (.kind w1 :: Γ') ★ w2 _ _ _ c3
+  case _ => apply Judgment.wfkind; apply compile_preserves_kinds wf h1 c2; assumption
+  case _ => apply HsJudgment.ax; apply HsJudgment.wfkind; assumption; assumption
+  case _ => unfold compile_kind; rfl
+
+case _ A B j1' j2' ih1 ih2 =>
+  rw[Option.bind_eq_some] at c2;
+  cases c2; case _ w1 c2 =>
+  cases c2; case _ c2 c3 =>
+  rw[Option.bind_eq_some] at c3;
+  cases c3; case _ w2 c3 =>
+  cases c3; case _ c3 e =>
+  cases e;
+  have lem1 := compile_preserves_kinds wf j1 c1;
+  unfold compile_kind at c1; simp at c1;
+  cases j1; simp at c1; cases c1;
+  apply Judgment.arrow;
+  apply @ih1 Γ' ★ w1 wf _ _ c2;
+  case _ => apply HsJudgment.ax; assumption
+  case _ => unfold compile_kind; rfl
+
+  apply @ih2 (.empty::Γ') ★ w2 _ _ _ c3;
+  case _ => apply Judgment.wfempty; assumption;
+  case _ => apply HsJudgment.ax; apply HsJudgment.wfempty; assumption
+  case _ => unfold compile_kind; rfl
+
+case _ j1 _ j2 ih1 ih2 =>
+  rw[Option.bind_eq_some] at c2;
+  cases c2; case _ w1 c2 =>
+  cases c2; case _ c2 c3 =>
+  rw[Option.bind_eq_some] at c3;
+  cases c3; case _ w2 c3 =>
+  cases c3; case _ c3 e =>
+  cases e;
+  have lem1 := compile_preserves_kinds wf j1 c1;
+  unfold compile_kind at c1; simp at c1;
+  cases j1; simp at c1; cases c1;
+  case _ tl1 tl2 _ =>
+  apply Judgment.arrow;
+  apply @ih1 Γ' ★ w1 wf _ _ c2;
+  case _ => apply HsJudgment.ax; assumption
+  case _ => unfold compile_kind; rfl
+  apply @ih2 (.empty::Γ') ★ w2 _ _ _ c3
+  case _ => apply Judgment.wfempty; assumption
+  case _ => apply HsJudgment.ax; apply HsJudgment.wfempty; assumption
+  case _ => unfold compile_kind; rfl
+
+
+@[simp]
+abbrev CompilePreservesTypeShapeAll :  (v : HsVariant) -> Ctx HsTerm -> HsJudgmentArgs v -> Prop
+| .type => λ Γ => λ (τ, k) => ∀ wA wτ cτ,
+  τ = (`∀{wA} wτ) ->
+  k = `★ ->
+  (j3 : Γ ⊢τ τ : k) ->
+  compile_type Γ τ k j3 = .some cτ ->
+  ∃ A' τ', cτ = ∀[A']τ'
+| _ => λ _ => λ _ => true
+
+theorem comile_preserves_type_shape_all_lemma :
+  HsJudgment v Γ idx -> CompilePreservesTypeShapeAll v Γ idx
+ := by
+intro j; induction j <;> simp at *;
+intro wA wτ cτ e1 e2 j3 c3;
+cases j3; case _ hka hkb =>
+unfold compile_type at c3; simp at c3;
+rw[Option.bind_eq_some] at c3;
+cases c3; case _ A' c3 =>
+cases c3; case _ cA c4 =>
+rw[Option.bind_eq_some] at c4;
+cases c4; case _ B' c4 =>
+cases c4; case _ cB e =>
+cases e; simp;
+
+theorem compile_preserves_type_shape_all :
+  (j : Γ ⊢τ (`∀{A}τ) : `★) ->
+  compile_type Γ (`∀{A}τ) `★ j = .some cτ ->
+  ∃ A' τ', cτ = ∀[A']τ' := by
+intro j c;
+have lem := comile_preserves_type_shape_all_lemma j; simp at lem;
+apply @lem A τ cτ rfl rfl j c
+
+
+@[simp]
+abbrev CompilePreservesTypeShapeArrow :  (v : HsVariant) -> Ctx HsTerm -> HsJudgmentArgs v -> Prop
+| .type => λ Γ => λ (τ, k) => ∀ wA wB cτ,
+  τ = (.HsBind2 .arrow wA wB) ->
+  k = `★ ->
+  (j3 : Γ ⊢τ τ : k) ->
+  compile_type Γ τ k j3 = .some cτ ->
+  ∃ A' B', cτ = (A' -t> B')
+| _ => λ _ => λ _ => true
+
+theorem comile_preserves_type_shape_arrow_lemma :
+  HsJudgment v Γ idx -> CompilePreservesTypeShapeArrow v Γ idx
+ := by
+intro j; induction j <;> simp at *;
+intro wA wτ cτ e1 e2 j3 c3;
+cases j3; case _ hka hkb =>
+unfold compile_type at c3; simp at c3;
+rw[Option.bind_eq_some] at c3;
+cases c3; case _ A' c3 =>
+cases c3; case _ cA c4 =>
+rw[Option.bind_eq_some] at c4;
+cases c4; case _ B' c4 =>
+cases c4; case _ cB e =>
+cases e; simp;
+
+
+theorem compile_preserves_type_shape_arrow :
+  (j1 : Γ ⊢τ (A → B) : `★) ->
+  compile_type Γ (A → B) `★ j1 = .some cτ ->
+  ∃ (A' : Term)  (B' : Term) (j2 : Γ ⊢τ A : `★) (j3 : (.empty :: Γ) ⊢τ B : `★),
+        cτ = (A' -t> B')
+         ∧ (compile_type Γ A `★ j2 = .some A')
+         ∧ (compile_type (.empty::Γ) B `★ j3 = .some B')  := by
+intro j1 j2;
+unfold compile_type at j2; cases j1; simp at j2;
+rw[Option.bind_eq_some] at j2;
+cases j2; case _ A' j2 =>
+cases j2; case _ j2 j3 =>
+rw[Option.bind_eq_some] at j3;
+cases j3; case _ B' j3 =>
+cases j3; case _ j3 e =>
+cases e; case _ ja jb =>
+exists A'; exists B'; exists ja; exists jb;
