Hs/Metatheory/SubstitutionCompile.lean
@@ -14,3 +14,20 @@ theorem compile_beta_kind_type :
   compile_type Γ t A j2 = .some t' ->
   (j3 : Γ ⊢τ (b β[t]) : (B β[t])) ->
   compile_type Γ (b β[t]) (B β[t]) j3 = .some (b' β[t']) := by sorry
+
+
+theorem compile_beta_empty_type :
+  (j1 : (.empty::Γ) ⊢τ b : B) ->
+  compile_type (.empty::Γ) b B j1 = .some b' ->
+  (j2 : Γ ⊢τ t : A) ->
+  compile_type Γ t A j2 = .some t' ->
+  (j3 : Γ ⊢τ (b β[t]) : (B β[t])) ->
+  compile_type Γ (b β[t]) (B β[t]) j3 = .some (b' β[t']) := by sorry
+
+theorem compile_beta_empty_term :
+  (j1 : (.empty::Γ) ⊢τ b : B) ->
+  compile_type (.empty::Γ) b B j1 = .some b' ->
+  (j2 : Γ ⊢t t : A) ->
+  compile_term Γ t A j2 = .some t' ->
+  (j3 : Γ ⊢τ (b β[t]) : (B β[t])) ->
+  compile_type Γ (b β[t]) (B β[t]) j3 = .some (b' β[t']) := by sorry
